CBOR.Pulse.API.Det.Common.cbor_det_parse now requires the slice to only contain valid data, no suffix

src/cbor/pulse/raw/CBOR.Pulse.API.Det.Common.fst
@@ -136,27 +136,33 @@ let cbor_det_parse_aux
 = Seq.lemma_split v len;
   Classical.move_requires (SpecRaw.serialize_cbor_inj (SpecRaw.mk_det_raw_cbor v1) v1' v2) (Seq.slice v (len) (Seq.length v))
 
+let cbor_det_parse_aux1
+  (v1: Spec.cbor)
+: Lemma
+  (let s = Spec.cbor_det_serialize v1 in s == s `Seq.append` Seq.empty)
+= Seq.append_empty_r (Spec.cbor_det_serialize v1)
+
 inline_for_extraction noextract [@@noextract_to "krml"]
 ```pulse
 fn cbor_det_parse
   (input: S.slice U8.t)
-  (len: SZ.t)
   (#pm: perm)
   (#v: Ghost.erased (Seq.seq U8.t))
 requires
     (pts_to input #pm v ** pure (
-      exists v1 v2 . Ghost.reveal v == Spec.cbor_det_serialize v1 `Seq.append` v2 /\ SZ.v len == Seq.length (Spec.cbor_det_serialize v1)
+      exists v1 . Ghost.reveal v == Spec.cbor_det_serialize v1 /\ SZ.v (S.len input) == Seq.length (Spec.cbor_det_serialize v1)
     ))
 returns res: cbor_det_t
 ensures
     (exists* v' .
       cbor_det_match 1.0R res v' **
       Trade.trade (cbor_det_match 1.0R res v') (pts_to input #pm v) ** pure (
-        SZ.v len <= Seq.length v /\
-        Seq.slice v 0 (SZ.v len) == Spec.cbor_det_serialize v'
+        Ghost.reveal v == Spec.cbor_det_serialize v'
     ))
 {
-  Seq.lemma_split v (SZ.v len);
+  let len = S.len input;
+  S.pts_to_len input;
+  Classical.forall_intro cbor_det_parse_aux1;
   let res = Parse.cbor_parse input len;
   with v1' . assert (Raw.cbor_match 1.0R res v1');
   Classical.forall_intro_2 (cbor_det_parse_aux v (SZ.v len) v1');
